lecture4/parts/4-solution-key.dfy
@@ -1,0 +1,51 @@
+method CopyInt(a: nat) returns (b: nat)
+    // Uncomment to try the example
+    // requires a >= 0 // (technically redundant as a: nat)
+    ensures b == a
+{
+    var i: nat := a;
+    b := 0;
+    while i > 0
+        // Technically these were not needed
+        invariant i <= a
+        invariant b >= 0
+        invariant i >= 0
+        // The right invariant!
+        invariant a == b + i
+        // This also works
+        // invariant a - i == b
+    {
+        i := i - 1;
+        b := b + 1;
+    }
+    // What do I know here?
+}
+
+// Another one for the following poll
+method AddOne(a: nat) returns (b: nat)
+    // Uncomment to try the example
+    ensures b == a + 1
+{
+    b := 0;
+    while b < a + 1
+        invariant b <= a + 1
+    {
+        b := b + 1;
+    }
+}
+
+
+method Find(a: seq<int>, key: int) returns (index: int)
+    ensures 0 <= index < |a| ==> a[index] == key
+    ensures index == |a| ==> forall k :: 0 <= k < |a| ==> a[k] != key
+{
+    index := 0;
+    while (index < |a|) && (a[index] != key)
+        invariant index <= |a|
+        invariant forall k :: 0 <= k < index ==> a[k] != key
+    {
+        index := index + 1;
+    }
+    // We know that index == |a| OR a[index] == key
+    // We know that forall k :: 0 <= k < |a| ==> a[k] != key
+}
